\documentclass[14pt]{article}

% Packages
\usepackage{ezra}

% Title
\title{2019 A1}
\author{Ezra Guerrero Alvarez}

% Formatting
\setlength{\parindent}{0pt}

%document
\begin{document}
\maketitle
	
\section*{2019 A1}

\begin{statement}{2019 A1}
	Solve over $\ZZ$ the functional equation
	$f(2a) + 2f(b) = f(f(a+b))$.
\end{statement}
We claim the only solutions are $f(x)=2x+c$ for any integer $c$, which clearly work. Setting $(a,b)=(0,n)$ and $(1,n-1)$ we obtain
\[ f(0)+2f(n)=f(f(n))=f(2)+2f(n-1), \]
so $f(n)-f(n-1)=\frac{f(2)-f(0)}2$. Since the right hand side is a constant and $f\colon\ZZ\rightarrow\ZZ$, it follows that $f(x)=mx+c$. Then, substituting in the original equation we find $m=2$ and $c$ can be anything. $\blacksquare$
	
\end{document}
